iris/WpStartNew.v
@@ -51,7 +51,7 @@
 From Stdlib Require Import Eqdep_dec ZArith Lia.
 From stdpp Require Import gmap list list_monad bitvector.definitions bitvector.tactics.
 From iris.proofmode Require Import proofmode.
-From iris.base_logic.lib Require Import gen_heap.
+From iris.base_logic.lib Require Import gen_heap ghost_map.
 From iris.program_logic Require Import language weakestpre lifting.
 Require Import SailStdpp.ConcurrencyInterface SailStdpp.ConcurrencyInterfaceBuiltins SailStdpp.ConcurrencyInterfaceTypes SailStdpp.Operators_mwords.
 Require Import Riscv.rv64d_types Riscv.rv64d Riscv.riscv_extras.
@@ -1163,7 +1163,7 @@ Section WpStartThm.
     r ↦ᵣ{DfracOwn (1/2)} v -∗ r ↦ᵣ{DfracOwn (1/2)} v -∗ r ↦ᵣ v.
   Proof.
     rewrite /reg_pointsto. iIntros "H1 H2".
-    iDestruct (pointsto_combine with "H1 H2") as "[H _]".
+    iDestruct (ghost_map_elem_combine with "H1 H2") as "[H _]".
     rewrite dfrac_op_own Qp.half_half. iExact "H".
   Qed.
 
